Restore ChoiceType syntax helpers before wf

ChoiceType/theories/Syntax.v
@@ -53,6 +53,72 @@ Fixpoint plug_ctx (Δ : ctx_hole) (Γ : ctx) : ctx :=
   | CtxHoleSum   Δ1 Δ2  => CtxSum   (plug_ctx Δ1 Γ) (plug_ctx Δ2 Γ)
   end.
 
+(** ** Free variables in types and contexts *)
+
+Fixpoint fv_cty (τ : choice_ty) : aset :=
+match τ with
+| CTOver  _ φ     => qual_fv φ
+| CTUnder _ φ     => qual_fv φ
+| CTInter τ1 τ2   => fv_cty τ1 ∪ fv_cty τ2
+| CTUnion τ1 τ2   => fv_cty τ1 ∪ fv_cty τ2
+| CTSum   τ1 τ2   => fv_cty τ1 ∪ fv_cty τ2
+| CTArrow x τx τ  => fv_cty τx ∪ (fv_cty τ ∖ {[ x ]})
+| CTWand  x τx τ  => fv_cty τx ∪ (fv_cty τ ∖ {[ x ]})
+end.
+
+Fixpoint fv_ctx (Γ : ctx) : aset :=
+match Γ with
+| CtxEmpty        => ∅
+| CtxBind x τ    => fv_cty τ          (** x itself is a binder, not free *)
+| CtxComma Γ1 Γ2 => fv_ctx Γ1 ∪ fv_ctx Γ2
+| CtxStar  Γ1 Γ2 => fv_ctx Γ1 ∪ fv_ctx Γ2
+| CtxSum   Γ1 Γ2 => fv_ctx Γ1 ∪ fv_ctx Γ2
+end.
+
+#[global] Instance stale_cty_inst : Stale choice_ty := fv_cty.
+#[global] Instance stale_ctx_inst : Stale ctx       := fv_ctx.
+Arguments stale_cty_inst /.
+Arguments stale_ctx_inst /.
+
+(** ** Type erasure and lifting *)
+
+(** [erase_ty τ] : the basic type underlying τ (Definition Fig. 2). *)
+Fixpoint erase_ty (τ : choice_ty) : ty :=
+  match τ with
+  | CTOver  b _     => TBase b
+  | CTUnder b _     => TBase b
+  | CTInter τ1 _    => erase_ty τ1
+  | CTUnion τ1 _    => erase_ty τ1
+  | CTSum   τ1 _    => erase_ty τ1
+  | CTArrow _ τx τ  => erase_ty τx →ₜ erase_ty τ
+  | CTWand  _ τx τ  => erase_ty τx →ₜ erase_ty τ
+  end.
+
+(** [lift_ty s] : lift a basic type to the default over-refinement type. *)
+Fixpoint lift_ty (s : ty) : choice_ty :=
+  match s with
+  | TBase b        => CTOver b qual_top   (** {ν:b | ⊤} *)
+  | TArrow s1 s2   =>
+      let τ1 := lift_ty s1 in
+      let τ2 := lift_ty s2 in
+      let x := fresh_for (fv_cty τ1 ∪ fv_cty τ2) in
+      CTArrow x τ1 τ2
+  end.
+
+(** [erase_ctx Γ] : the basic context underlying Γ. *)
+Fixpoint erase_ctx (Γ : ctx) : gmap atom ty :=
+  match Γ with
+  | CtxEmpty        => ∅
+  | CtxBind x τ    => {[ x := erase_ty τ ]}
+  | CtxComma Γ1 Γ2 => erase_ctx Γ1 ∪ erase_ctx Γ2
+  | CtxStar  Γ1 Γ2 => erase_ctx Γ1 ∪ erase_ctx Γ2
+  | CtxSum   Γ1 _  => erase_ctx Γ1
+  end.
+
+(** [lift_ctx Γ_basic] : lift a basic context. *)
+Definition lift_ctx (Γ : gmap atom ty) : ctx :=
+  map_fold (fun x s acc => CtxComma (CtxBind x (lift_ty s)) acc) CtxEmpty Γ.
+
 (** ** Domain (free variables from binders) *)
 
 Fixpoint ctx_dom (Γ : ctx) : aset :=
